new/golang/theory/typing.v
@@ -21,12 +21,12 @@ Section goose_lang.
 
   Infix "=?" := (String.eqb).
 
-  Definition val_def (t : go_type) (field_vals: gmap string val): val :=
+  Definition val_def (t : go_type) (field_vals: list (string*val)): val :=
     match t with
     | structT d => (fix val_struct (fs : list (string*go_type)) :=
                      match fs with
                      | [] => (#())
-                     | (f,ft)::fs => (default (zero_val ft) (field_vals !! f), val_struct fs)%V
+                     | (f,ft)::fs => (default (zero_val ft) (assocl_lookup f field_vals), val_struct fs)%V
                      end) d
     | _ => LitV LitPoison
     end.
@@ -106,7 +106,7 @@ Section typing.
 
   | has_go_type_struct
       (d : struct.descriptor) fvs
-      (Hfields : ∀ f t, In (f, t) d → has_go_type (default (zero_val t) (fvs !! f)) t)
+      (Hfields : ∀ f t, In (f, t) d → has_go_type (default (zero_val t) (assocl_lookup f fvs)) t)
     : has_go_type (struct.val (structT d) fvs) (structT d)
   | has_go_type_ptr (l : loc) : has_go_type #l ptrT
   | has_go_type_func f e v : has_go_type (RecV f e v) funcT
@@ -124,7 +124,7 @@ Section typing.
     has_go_type (zero_val t) t.
   Proof.
     induction t using go_type_ind; rewrite zero_val_unseal; try econstructor.
-    replace (zero_val_def (structT decls)) with (struct.val (structT decls) ∅).
+    replace (zero_val_def (structT decls)) with (struct.val (structT decls) []).
     {
       econstructor. intros. simpl.
       apply Hfields.
@@ -177,7 +177,7 @@ Section typing.
     | stringT => #(str "")
     (* | arrayT (len : nat) (elem : go_type) *)
     | sliceT _ => slice.nil
-    | structT decls => struct.val t ∅
+    | structT decls => struct.val t []
     | ptrT => nil
     | funcT => nil
     | interfaceT => interface_nil
